Done simplifying #208

examples/bug-reports/bug208.fst
@@ -1,12 +1,11 @@
 module Bug208
 
-assume type acc (a:Type) (r:(a -> a -> Type)) (x:a) : Type
+assume type acc (r:(int -> Type)) : Type
 
-assume val acc_inv : r:('a -> 'a -> Type) -> x:'a -> a:(acc 'a r x) ->
-              Tot (y:'a -> r y x -> Tot (acc 'a r y))
+assume val acc_inv : r:(int -> Type) -> acc r ->
+              Tot (y:int -> Tot (r y))
 
-assume val axiom1 : #a:Type -> #b:Type -> f:(a -> Tot b) -> Lemma True
+assume val axiom1 : #b:Type -> f:(int -> Tot b) -> Lemma True
 
-val fix_F : r:(int -> int -> Type) ->
-            x:int -> acc int r x -> Tot unit
-let rec fix_F x a = axiom1 (acc_inv x a)
+val fix_F : r:(int -> Type) -> acc r -> Tot unit
+let rec fix_F a = axiom1 (acc_inv a)
