examples/bug-reports/bug128.fst
@@ -1,4 +1,4 @@
-module Bug123
+module Bug128
 
 val subst : x:int -> Tot unit (decreases (if x = 42 then LexTop else LexTop))
 let rec subst x = ()
